Add [freeze] to Arithmetic

src/Experiments/NewPipeline/Arithmetic.v
@@ -16,6 +16,7 @@ Require Import Crypto.Util.Tactics.RunTacticAsConstr.
 Require Import Crypto.Util.Tactics.Head.
 Require Import Crypto.Util.Option.
 Require Import Crypto.Util.OptionList.
+Require Import Crypto.Util.Prod.
 Require Import Crypto.Util.Sum.
 Require Import Crypto.Util.ZUtil.
 Require Import Crypto.Util.ZUtil.Modulo Crypto.Util.ZUtil.Div Crypto.Util.ZUtil.Hints.Core.
@@ -459,9 +460,62 @@ Module Positional. Section Positional.
   End sub.
   Hint Rewrite @eval_opp @eval_sub : push_eval.
   Hint Rewrite @length_sub @length_opp : distr_length.
+
+  Section select.
+    Definition select (mask cond:Z) (p:list Z) :=
+      dlet t := Z.zselect cond 0 mask in List.map (Z.land t) p.
+
+    Lemma map_and_0 n (p:list Z) : length p = n -> map (Z.land 0) p = zeros n.
+    Proof.
+      intro; subst; induction p as [|x xs IHxs]; [reflexivity | ].
+      cbn; f_equal; auto.
+    Qed.
+    Lemma eval_select n mask cond p (H:List.map (Z.land mask) p = p) :
+      length p = n
+      -> eval n (select mask cond p) =
+         if dec (cond = 0) then 0 else eval n p.
+    Proof.
+      cbv [select Let_In].
+      rewrite Z.zselect_correct; break_match.
+      { intros; erewrite map_and_0 by eassumption. apply eval_zeros. }
+      { rewrite H; reflexivity. }
+    Qed.
+    Lemma length_select mask cond p :
+      length (select mask cond p) = length p.
+    Proof using Type. clear dependent weight. cbv [select Let_In]; break_match; intros; distr_length. Qed.
+  End select.
 End Positional.
 (* Hint Rewrite disappears after the end of a section *)
-Hint Rewrite length_zeros length_add_to_nth length_from_associational @length_add @length_carry_reduce @length_chained_carries @length_encode @length_sub @length_opp : distr_length.
+Hint Rewrite length_zeros length_add_to_nth length_from_associational @length_add @length_carry_reduce @length_chained_carries @length_encode @length_sub @length_opp @length_select : distr_length.
+Hint Rewrite @eval_select : push_eval.
+Section Positional_nonuniform.
+  Context (weight weight' : nat -> Z).
+
+  Lemma eval_hd_tl n (xs:list Z) :
+    length xs = n ->
+    eval weight n xs = weight 0%nat * hd 0 xs + eval (fun i => weight (S i)) (pred n) (tl xs).
+  Proof.
+    intro; subst; destruct xs as [|x xs]; [ cbn; omega | ].
+    cbv [eval to_associational Associational.eval] in *; cbn.
+    rewrite <- map_S_seq; reflexivity.
+  Qed.
+
+  Lemma eval_cons n (x:Z) (xs:list Z) :
+    length xs = n ->
+    eval weight (S n) (x::xs) = weight 0%nat * x + eval (fun i => weight (S i)) n xs.
+  Proof. intro; subst; apply eval_hd_tl; reflexivity. Qed.
+
+  Lemma eval_weight_mul n p k :
+    (forall i, In i (seq 0 n) -> weight i = k * weight' i) ->
+    eval weight n p = k * eval weight' n p.
+  Proof.
+    setoid_rewrite List.in_seq.
+    revert n weight weight'; induction p as [|x xs IHxs], n as [|n]; intros weight weight' Hwt;
+      cbv [eval to_associational Associational.eval] in *; cbn in *; try omega.
+    rewrite Hwt, Z.mul_add_distr_l, Z.mul_assoc by omega.
+    erewrite <- !map_S_seq, IHxs; [ reflexivity | ]; cbn; eauto with omega.
+  Qed.
+End Positional_nonuniform.
 End Positional.
 
 Record weight_properties {weight : nat -> Z} :=
@@ -1006,7 +1060,6 @@ Module Columns.
       Qed. Hint Rewrite eval_cons_to_nth using (solve [distr_length]) : push_eval.
 
       Hint Rewrite Positional.eval_zeros : push_eval.
-      Hint Rewrite Positional.length_from_associational : distr_length.
       Hint Rewrite Positional.eval_add_to_nth using (solve [distr_length]): push_eval.
 
       (* from_associational *)
@@ -1108,13 +1161,13 @@ Module Rows.
         destruct x; cbn [hd tl]; rewrite ?sum_nil, ?sum_cons; ring.
       Qed. Hint Rewrite eval_extract_row using (solve [distr_length]) : push_eval.
 
-      Lemma length_fst_extract_row n (inp : cols) :
-        length inp = n -> length (fst (extract_row inp)) = n.
+      Lemma length_fst_extract_row (inp : cols) :
+        length (fst (extract_row inp)) = length inp.
       Proof. cbv [extract_row]; autorewrite with cancel_pair; distr_length. Qed.
       Hint Rewrite length_fst_extract_row : distr_length.
 
-      Lemma length_snd_extract_row n (inp : cols) :
-        length inp = n -> length (snd (extract_row inp)) = n.
+      Lemma length_snd_extract_row (inp : cols) :
+        length (snd (extract_row inp)) = length inp.
       Proof. cbv [extract_row]; autorewrite with cancel_pair; distr_length. Qed.
       Hint Rewrite length_snd_extract_row : distr_length.
 
@@ -1169,7 +1222,8 @@ Module Rows.
                  | _ => progress In_cases
                  | _ => split; try omega
                  | H: _ /\ _ |- _ => destruct H
-                 | _ => solve [auto using length_fst_extract_row, length_snd_extract_row]
+                 | _ => progress distr_length
+                 | _ => solve [auto]
                  end.
       Qed.
       Lemma length_fst_from_columns' m st :
@@ -1227,7 +1281,7 @@ Module Rows.
         eapply length_snd_from_columns'; eauto.
         autorewrite with cancel_pair; intros; In_cases.
       Qed.
-      Hint Rewrite length_from_columns : distr_length.
+      Hint Rewrite length_from_columns using eassumption : distr_length.
 
       (* from associational *)
       Definition from_associational n (p : list (Z * Z)) := from_columns (Columns.from_associational weight n p).
@@ -1513,7 +1567,7 @@ Module Rows.
       Lemma flatten_div_mod inp n :
         (forall row, In row inp -> length row = n) ->
         is_div_mod (Positional.eval weight n) (flatten n inp) (eval n inp) (weight n).
-      Proof.
+      Proof using wprops.
         intros; cbv [flatten].
         destruct inp; [|destruct inp]; cbn [hd tl].
         { cbv [is_div_mod]; push.
@@ -1556,7 +1610,7 @@ Module Rows.
         forall i, (i < n)%nat ->
                   nth_default 0 (fst (flatten' start_state inp)) i
                   = ((Positional.eval weight n (fst start_state) + eval n inp) mod weight (S i)) / (weight i).
-      Proof.
+      Proof using wprops.
         induction inp using rev_ind; push.
         destruct (dec (inp = nil)).
         { subst inp; push. rewrite sum_rows_partitions with (n:=n) by eauto. push. }
@@ -1569,7 +1623,7 @@ Module Rows.
         (forall row, In row inp -> length row = n) ->
         forall i, (i < n)%nat ->
                   nth_default 0 (fst (flatten n inp)) i = (eval n inp mod weight (S i)) / (weight i).
-      Proof.
+      Proof using wprops.
         intros; cbv [flatten].
         intros; destruct inp as [| ? [| ? ?] ]; try congruence; cbn [hd tl] in *;  try solve [push].
         { cbn. autorewrite with push_nth_default.
@@ -1587,7 +1641,7 @@ Module Rows.
         (forall i, (i < n)%nat -> nth_default 0 p i = (x mod weight (S i)) / weight i) ->
         length p = n ->
         p = partition n x.
-      Proof.
+      Proof using Type.
         cbv [partition]; induction p using rev_ind; intros; distr_length; subst n; [reflexivity|].
         rewrite Nat.add_1_r, seq_snoc.
         autorewrite with natsimplify push_map.
@@ -1601,18 +1655,18 @@ Module Rows.
 
       Lemma partition_step n x :
         partition (S n) x = partition n x ++ [(x mod weight (S n)) / weight n].
-      Proof.
+      Proof using Type.
         cbv [partition]. rewrite seq_snoc.
         autorewrite with natsimplify push_map. reflexivity.
       Qed.
 
       Lemma length_partition n x : length (partition n x) = n.
-      Proof. cbv [partition]; distr_length. Qed.
+      Proof using Type. cbv [partition]; distr_length. Qed.
       Hint Rewrite length_partition : distr_length.
 
       Lemma eval_partition n x :
         Positional.eval weight n (partition n x) = x mod (weight n).
-      Proof.
+      Proof using wprops.
         induction n; intros.
         { cbn. rewrite (weight_0); auto with zarith. }
         { rewrite (Z.div_mod (x mod weight (S n)) (weight n)) by auto.
@@ -1621,10 +1675,26 @@ Module Rows.
           omega. }
       Qed.
 
+      Lemma partition_Proper n :
+        Proper (Z.equiv_modulo (weight n) ==> eq) (partition n).
+      Proof using wprops.
+        cbv [Proper Z.equiv_modulo respectful].
+        intros x y Hxy; induction n; intros.
+        { reflexivity. }
+        { assert (Hxyn : x mod weight n = y mod weight n).
+          { erewrite (Znumtheory.Zmod_div_mod _ (weight (S n)) x), (Znumtheory.Zmod_div_mod _ (weight (S n)) y), Hxy
+              by (try apply Z.mod_divide; auto);
+              reflexivity. }
+          rewrite !partition_step, IHn by eauto.
+          rewrite (Z.div_mod (x mod weight (S n)) (weight n)), (Z.div_mod (y mod weight (S n)) (weight n)) by auto.
+          rewrite <-!Znumtheory.Zmod_div_mod by (try apply Z.mod_divide; auto).
+          rewrite Hxy, Hxyn; reflexivity. }
+      Qed.
+
       Lemma flatten_partitions' inp n :
         (forall row, In row inp -> length row = n) ->
         fst (flatten n inp) = partition n (eval n inp).
-      Proof. auto using nth_default_partitions, flatten_partitions, length_flatten. Qed.
+      Proof using wprops. auto using nth_default_partitions, flatten_partitions, length_flatten. Qed.
     End Flatten.
 
     Section Ops.
@@ -1638,6 +1708,10 @@ Module Rows.
       NOTE(from jgross): I think partial evaluation now handles that
       fine; we should check this. *)
       Definition sub n p q := flatten n [p; map (fun x => dlet y := x in Z.opp y) q].
+
+      Definition conditional_add n mask cond (p q:list Z) :=
+        let qq := Positional.select mask cond q in
+        add n p qq.
 
       Hint Rewrite eval_cons eval_nil using solve [auto] : push_eval.
 
@@ -1675,17 +1749,34 @@ Module Rows.
       Lemma add_partitions n p q :
         n <> 0%nat -> length p = n -> length q = n ->
         fst (add n p q) = partition n (Positional.eval weight n p + Positional.eval weight n q).
-      Proof. solver. Qed.
+      Proof using wprops. solver. Qed.
 
       Lemma add_div n p q :
         n <> 0%nat -> length p = n -> length q = n ->
         snd (add n p q) = (Positional.eval weight n p + Positional.eval weight n q) / weight n.
-      Proof. solver. Qed.
+      Proof using wprops. solver. Qed.
+
+      Lemma conditional_add_partitions n mask cond p q :
+        n <> 0%nat -> length p = n -> length q = n -> map (Z.land mask) q = q ->
+        fst (conditional_add n mask cond p q)
+        = partition n (Positional.eval weight n p + if dec (cond = 0) then 0 else Positional.eval weight n q).
+      Proof using wprops.
+        cbv [conditional_add]; intros; rewrite add_partitions by (distr_length; auto).
+        autorewrite with push_eval; auto.
+      Qed.
+
+      Lemma conditional_add_div n mask cond p q :
+        n <> 0%nat -> length p = n -> length q = n -> map (Z.land mask) q = q ->
+        snd (conditional_add n mask cond p q) = (Positional.eval weight n p + if dec (cond = 0) then 0 else Positional.eval weight n q) / weight n.
+      Proof using wprops.
+        cbv [conditional_add]; intros; rewrite add_div by (distr_length; auto).
+        autorewrite with push_eval; auto.
+      Qed.
 
       Lemma eval_map_opp q :
         forall n, length q = n ->
                   Positional.eval weight n (map Z.opp q) = - Positional.eval weight n q.
-      Proof.
+      Proof using Type.
         induction q using rev_ind; intros;
           repeat match goal with
                  | _ => progress autorewrite with push_map push_eval
@@ -1698,23 +1789,23 @@ Module Rows.
       Lemma sub_partitions n p q :
         n <> 0%nat -> length p = n -> length q = n ->
         fst (sub n p q) = partition n (Positional.eval weight n p - Positional.eval weight n q).
-      Proof. solver. Qed.
+      Proof using wprops. solver. Qed.
 
       Lemma sub_div n p q :
         n <> 0%nat -> length p = n -> length q = n ->
         snd (sub n p q) = (Positional.eval weight n p - Positional.eval weight n q) / weight n.
-      Proof. solver. Qed.
+      Proof using wprops. solver. Qed.
 
       Lemma mul_partitions base n m p q :
         base <> 0 -> n <> 0%nat -> m <> 0%nat -> length p = n -> length q = n ->
         fst (mul base n m p q) = partition m (Positional.eval weight n p * Positional.eval weight n q).
-      Proof. solver. Qed.
+      Proof using wprops. solver. Qed.
 
       Lemma eval_sat_reduce base s c p :
         base <> 0 -> s - Associational.eval c <> 0 -> s <> 0 ->
         Associational.eval (sat_reduce base s c p) mod (s - Associational.eval c)
         = Associational.eval p mod (s - Associational.eval c).
-      Proof.
+      Proof using Type.
         intros; cbv [sat_reduce].
         autorewrite with push_eval.
         rewrite <-Associational.reduction_rule by omega.
@@ -1726,7 +1817,7 @@ Module Rows.
         base <> 0 -> s - Associational.eval c <> 0 -> s <> 0 ->
         Associational.eval (repeat_sat_reduce base s c p n) mod (s - Associational.eval c)
         = Associational.eval p mod (s - Associational.eval c).
-      Proof.
+      Proof using Type.
         intros; cbv [repeat_sat_reduce].
         apply fold_right_invariant; intros; autorewrite with push_eval; auto.
       Qed.
@@ -1738,13 +1829,16 @@ Module Rows.
         (Positional.eval weight n (fst (mulmod base s c n nreductions p q))
          + weight n * (snd (mulmod base s c n nreductions p q))) mod (s - Associational.eval c)
         = (Positional.eval weight n p * Positional.eval weight n q) mod (s - Associational.eval c).
-      Proof.
+      Proof using wprops.
         solver.
         rewrite <-Z.div_mod'' by auto.
         autorewrite with push_eval; reflexivity.
       Qed.
     End Ops.
   End Rows.
+  Hint Rewrite length_from_columns using eassumption : distr_length.
+  Hint Rewrite length_sum_rows using solve [ reflexivity | eassumption | distr_length; eauto ] : distr_length.
+  Hint Rewrite length_fst_extract_row length_snd_extract_row length_flatten length_flatten' length_partition length_fst_from_columns' length_snd_from_columns' : distr_length.
 End Rows.
 
 Module BaseConversion.
@@ -1762,7 +1856,7 @@ Module BaseConversion.
     Lemma eval_convert_bases sn dn p :
       (dn <> 0%nat) -> length p = sn ->
       eval dw dn (convert_bases sn dn p) = eval sw sn p.
-    Proof.
+    Proof using dwprops.
       cbv [convert_bases]; intros.
       rewrite eval_chained_carries_no_reduce; auto using ZUtil.Z.positive_is_nonzero.
       rewrite eval_from_associational; auto.
@@ -1792,7 +1886,7 @@ Module BaseConversion.
 
       Lemma eval_reordering_carry w fw p (_:fw<>0):
         Associational.eval (reordering_carry w fw p) = Associational.eval p.
-      Proof.
+      Proof using Type.
         cbv [reordering_carry]. induction p; [reflexivity |].
         autorewrite with push_fold_right. break_match; push_eval.
       Qed.
@@ -1814,13 +1908,13 @@ Module BaseConversion.
     Lemma eval_to_associational n m p :
       m <> 0%nat -> length p = n ->
       Associational.eval (to_associational n m p) = Positional.eval sw n p.
-    Proof. cbv [to_associational]; push_eval. Qed.
+    Proof using dwprops. cbv [to_associational]; push_eval. Qed.
     Hint Rewrite eval_to_associational using solve [push_eval; distr_length] : push_eval.
 
     Lemma eval_from_associational idxs n p :
       n <> 0%nat -> 0 <= Associational.eval p < sw n ->
       Positional.eval sw n (from_associational idxs n p) = Associational.eval p.
-    Proof.
+    Proof using dwprops swprops.
       cbv [from_associational]; intros.
       rewrite Rows.flatten_mod by eauto using Rows.length_from_associational.
       rewrite Associational.bind_snd_correct.
@@ -1831,7 +1925,7 @@ Module BaseConversion.
     Lemma from_associational_partitions n idxs p  (_:n<>0%nat):
       forall i, (i < n)%nat ->
                 nth_default 0 (from_associational idxs n p) i = (Associational.eval p) mod (sw (S i)) / sw i.
-    Proof.
+    Proof using dwprops swprops.
       intros; cbv [from_associational].
       rewrite Rows.flatten_partitions with (n:=n) by (eauto using Rows.length_from_associational; omega).
       rewrite Associational.bind_snd_correct.
@@ -1840,7 +1934,7 @@ Module BaseConversion.
 
     Lemma from_associational_eq n idxs p  (_:n<>0%nat):
       from_associational idxs n p = Rows.partition sw n (Associational.eval p).
-    Proof.
+    Proof using dwprops swprops.
       intros. cbv [from_associational].
       rewrite Rows.flatten_partitions' with (n:=n) by eauto using Rows.length_from_associational.
       rewrite Associational.bind_snd_correct.
@@ -1898,13 +1992,13 @@ Module BaseConversion.
         length p1 = n1 -> length p2 = n2 ->
         0 <= (Positional.eval sw n1 p1 * Positional.eval sw n2 p2) < sw n3 ->
         Positional.eval sw n3 (mul_converted n1 n2 m1 m2 n3 idxs p1 p2) = (Positional.eval sw n1 p1) * (Positional.eval sw n2 p2).
-      Proof.  cbv [mul_converted]; push_eval. Qed.
+      Proof using dwprops swprops. cbv [mul_converted]; push_eval. Qed.
       Hint Rewrite eval_mul_converted : push_eval.
 
       Lemma mul_converted_partitions n1 n2 m1 m2 n3 idxs p1 p2  (_:n3<>0%nat) (_:m1<>0%nat) (_:m2<>0%nat):
         length p1 = n1 -> length p2 = n2 ->
         mul_converted n1 n2 m1 m2 n3 idxs p1 p2 = Rows.partition sw n3 (Positional.eval sw n1 p1 * Positional.eval sw n2 p2).
-      Proof.
+      Proof using dwprops swprops.
         intros; cbv [mul_converted].
         rewrite from_associational_eq by auto. push_eval.
       Qed.
@@ -1931,7 +2025,7 @@ Module BaseConversion.
     Lemma widemul_correct a b :
       0 <= a * b < 2^log2base * 2^log2base ->
       widemul a b = [(a * b) mod 2^log2base; (a * b) / 2^log2base].
-    Proof.
+    Proof using dwprops swprops.
       cbv [widemul]; intros.
       rewrite mul_converted_partitions by auto with zarith.
       subst nout sw; cbv [weight]; cbn.
@@ -1980,3 +2074,114 @@ Module BaseConversion.
     Qed.
   End widemul.
 End BaseConversion.
+
+(* TODO: rename this module? (Should it be, e.g., [Rows.freeze]?) *)
+Module Freeze.
+  Section Freeze.
+    Context weight {wprops : @weight_properties weight}.
+
+    Definition freeze n mask (m p:list Z) : list Z :=
+      let '(p, carry) := Rows.sub weight n p m in
+      let '(r, carry) := Rows.conditional_add weight n mask carry p m in
+      r.
+
+    Lemma freezeZ m s c y :
+      m = s - c ->
+      0 < c < s ->
+      s <> 0 ->
+      0 <= y < 2*m ->
+      ((y - m) + (if (dec ((y - m) / s = 0)) then 0 else m)) mod s
+      = y mod m.
+    Proof using Type.
+      clear; intros.
+      transitivity ((y - m) mod m);
+        repeat first [ progress intros
+                     | progress subst
+                     | break_innermost_match_step
+                     | progress autorewrite with zsimplify_fast
+                     | rewrite Z.div_small_iff in * by auto
+                     | progress (Z.rewrite_mod_small; push_Zmod; Z.rewrite_mod_small)
+                     | progress destruct_head'_or
+                     | omega ].
+    Qed.
+
+    Lemma length_freeze n mask m p :
+      length m = n -> length p = n -> length (freeze n mask m p) = n.
+    Proof using wprops.
+      cbv [freeze Rows.conditional_add Rows.add]; eta_expand; intros.
+      distr_length; try assumption; cbn; intros; destruct_head'_or; destruct_head' False; subst;
+        distr_length.
+      erewrite Rows.length_sum_rows by (reflexivity || eassumption || distr_length); distr_length.
+    Qed.
+    Lemma eval_freeze_eq n mask m p
+          (n_nonzero:n<>0%nat)
+          (Hmask : List.map (Z.land mask) m = m)
+          (Hplen : length p = n)
+          (Hmlen : length m = n)
+      : Positional.eval weight n (@freeze n mask m p)
+        = (Positional.eval weight n p - Positional.eval weight n m +
+           (if dec ((Positional.eval weight n p - Positional.eval weight n m) / weight n = 0) then 0 else Positional.eval weight n m))
+            mod weight n.
+            (*if dec ((Positional.eval weight n p - Positional.eval weight n m) / weight n = 0)
+          then Positional.eval weight n p - Positional.eval weight n m
+          else Positional.eval weight n p mod weight n.*)
+    Proof using wprops.
+      pose proof (@weight_positive weight wprops n).
+      cbv [freeze Z.equiv_modulo]; eta_expand.
+      repeat first [ solve [auto]
+                   | rewrite Rows.conditional_add_partitions
+                   | rewrite Rows.sub_partitions
+                   | rewrite Rows.sub_div
+                   | rewrite Rows.eval_partition
+                   | progress distr_length
+                   | progress pull_Zmod (*
+                   | progress break_innermost_match_step
+                   | progress destruct_head'_or
+                   | omega
+                   | f_equal; omega
+                   | rewrite Z.div_small_iff in * by (auto using (@weight_positive weight ltac:(assumption)))
+                   | progress Z.rewrite_mod_small *) ].
+    Qed.
+
+    Lemma eval_freeze n c mask m p
+          (n_nonzero:n<>0%nat)
+          (Hc : 0 < Associational.eval c < weight n)
+          (Hmask : List.map (Z.land mask) m = m)
+          modulus (Hm : Positional.eval weight n m = Z.pos modulus)
+          (Hp : 0 <= Positional.eval weight n p < 2*(Z.pos modulus))
+          (Hsc : Z.pos modulus = weight n - Associational.eval c)
+          (Hplen : length p = n)
+          (Hmlen : length m = n)
+      : Positional.eval weight n (@freeze n mask m p)
+        = Positional.eval weight n p mod (Z.pos modulus).
+    Proof using wprops.
+      pose proof (@weight_positive weight wprops n).
+      rewrite eval_freeze_eq by assumption.
+      erewrite freezeZ; try eassumption; try omega.
+      f_equal; omega.
+    Qed.
+
+    Lemma freeze_partitions n c mask m p
+          (n_nonzero:n<>0%nat)
+          (Hc : 0 < Associational.eval c < weight n)
+          (Hmask : List.map (Z.land mask) m = m)
+          modulus (Hm : Positional.eval weight n m = Z.pos modulus)
+          (Hp : 0 <= Positional.eval weight n p < 2*(Z.pos modulus))
+          (Hsc : Z.pos modulus = weight n - Associational.eval c)
+          (Hplen : length p = n)
+          (Hmlen : length m = n)
+      : @freeze n mask m p = Rows.partition weight n (Positional.eval weight n p mod (Z.pos modulus)).
+    Proof using wprops.
+      pose proof (@weight_positive weight wprops n).
+      pose proof (fun v => Z.mod_pos_bound v (weight n) ltac:(lia)).
+      pose proof (Z.mod_pos_bound (Positional.eval weight n p) (Z.pos modulus) ltac:(lia)).
+      erewrite <- eval_freeze by eassumption.
+      cbv [freeze]; eta_expand.
+      rewrite Rows.conditional_add_partitions by (auto; rewrite Rows.sub_partitions; auto; distr_length).
+      rewrite !Rows.eval_partition by assumption.
+      apply Rows.partition_Proper; [ assumption .. | ].
+      cbv [Z.equiv_modulo].
+      pull_Zmod; reflexivity.
+    Qed.
+  End Freeze.
+End Freeze.
